w_rules

WPDS/WEx.thy
@@ -23,12 +23,24 @@ lift_definition q2 :: state is 1 by auto
 lift_definition qf :: state is 2 by auto
 
 (* Define rules of PDS, and the two P-automata *)
-definition pds_rules :: "(ctr_loc, label, nat_inf) rule set" where
-  "pds_rules = {
+definition wpds_rules :: "(ctr_loc, label, nat_inf) w_rule set" where
+  "wpds_rules = {
   ((p1, y), fin 1,(p1, push x y)),
   ((p1, x), fin 2,(p2, swap y)),
   ((p2, x), fin 3,(p3, pop)),
   ((p3, y), fin 4,(p2, swap x))}"
+definition pds_rules :: "(ctr_loc, label) rule set" where
+  "pds_rules = {
+  ((p1, y), (p1, push x y)),
+  ((p1, x), (p2, swap y)),
+  ((p2, x), (p3, pop)),
+  ((p3, y), (p2, swap x))}"
+definition W :: "(ctr_loc, label) rule \<Rightarrow> nat_inf" where
+  "W rule = (K$ infinity)
+    (((p1, y), (p1, push x y)) $:= fin 1)
+    (((p1, x), (p2, swap y))   $:= fin 2)
+    (((p2, x), (p3, pop))      $:= fin 3)
+    (((p3, y), (p2, swap x))   $:= fin 4) $ rule"
 
 definition initial_automaton :: "((ctr_loc, state) WPDS2.state, label) transition set" where
   "initial_automaton = {
@@ -42,6 +54,9 @@ definition final_automaton :: "((ctr_loc, state) WPDS2.state, label) transition 
   ((Init p2, y, Noninit q1)),
   ((Init p3, x, Noninit q1)),
   ((Noninit q1, y, Noninit q2))}"
+
+definition "initial_finals = {Noninit qf}"
+definition "final_finals = {Noninit q2}"
 
 definition final_ctr_loc where "final_ctr_loc = {}"
 definition final_ctr_loc_st where "final_ctr_loc_st = {q2}"
@@ -156,26 +171,35 @@ end
 
 
 
+lemma "wpds_rules = w_rules pds_rules W"
+  unfolding pds_rules_def W_def wpds_rules_def w_rules_def by eval
 
 
-term "thing2 pds_rules initial_automaton final_automaton final_ctr_loc initial_ctr_loc"
+term "thing2 pds_rules W initial_automaton final_automaton initial_finals final_finals"
 
 
-
+lemma[code_unfold]: "finite pds_rules"
+  by simp
+  (*unfolding pds_rules_def
+  by simp
+ 
+value "finite pds_rules"*)
 
 (* The check function agrees with the encoded answer (Some True) 
    and therefore the proof succeeds as expected. *)
 
-definition "thing3 == thing2 pds_rules initial_automaton final_automaton initial_ctr_loc final_ctr_loc = Some (fin 20)"
+definition "thing3 == thing2 pds_rules W initial_automaton final_automaton initial_finals final_finals"
 
-export_code thing3 in Haskell (* nat_inf :: enum is not a reasonable requirement *)
+export_code thing3 in Haskell module_name WPDS_Example
+
+value "thing3"
 
 lemma
-  "thing2 pds_rules initial_automaton final_automaton initial_ctr_loc final_ctr_loc = Some (fin 20)"
+  "thing3 = Some (fin 5)"
   by code_simp
 
 lemma
-  "thing2 pds_rules initial_automaton final_automaton initial_ctr_loc final_ctr_loc = Some (fin 20)"
+  "thing3 = Some (fin 5)"
   by eval (* nat_inf :: enum is not a reasonable requirement *)
 
 end
